## Question 1

*(a)* **True.** If two sets of variables are jointly Gaussian, the conditional distribution of one set conditioned on the other is indeed Gaussian. Similarly, the marginal distribution of either set is also Gaussian.

*(b)* When we have a multivariate Gaussian distribution and we want to find the conditional distribution of one subset of variables given another, the formula for the conditional mean and conditional covariance are as follows:

Given 
$$
x = \begin{bmatrix} x_a \\ x_b \\ x_c \end{bmatrix}, \quad
\mu = \begin{bmatrix} \mu_a \\ \mu_b \\ \mu_c \end{bmatrix}
$$
and
$$
\Sigma = 
\begin{bmatrix} 
\Sigma_{aa} & \Sigma_{ab} & \Sigma_{ac} \\ 
\Sigma_{ba} & \Sigma_{bb} & \Sigma_{bc} \\ 
\Sigma_{ca} & \Sigma_{cb} & \Sigma_{cc} 
\end{bmatrix}
$$
The conditional distribution $p(x_a | x_b)$ is Gaussian with:

Mean:
$$
\mu_{a|b} = \mu_a + \Sigma_{ab} \Sigma_{bb}^{-1} (x_b - \mu_b)
$$
Covariance:
$$
\Sigma_{a|b} = \Sigma_{aa} - \Sigma_{ab} \Sigma_{bb}^{-1} \Sigma_{ba}
$$
So the conditional distribution $p(x_a | x_b)$ is:
$$
p(x_a | x_b) \sim \mathcal{N}(\mu_{a|b}, \Sigma_{a|b})
$$
Where $\mathcal{N}(\mu, \Sigma)$ denotes the Gaussian distribution with mean $\mu$ and covariance matrix $\Sigma$.



## Question 2

#### (a) Marginal Distribution $p(x)$

From the given joint distribution's mean and covariance matrix, we can observe:
$$
\mathrm{cov}[\mathbf{z}] = 
\left( 
\begin{array}{cc}
\mathbf{\Sigma}_{xx} & \mathbf{\Sigma}_{xy} \\
\mathbf{\Sigma}_{yx} & \mathbf{\Sigma}_{yy}
\end{array} 
\right) = 
\left( \begin{array}{cc} 
\mathbf{\Lambda^{-1}} & \mathbf{\Lambda^{-1}A^\mathrm{T}} \\
\mathbf{A\Lambda^{-1}} & \mathbf{L^{-1}+A\Lambda^{-1}A^\mathrm{T}}
\end{array} \right)
$$

$$
\mathbb{E}[\mathbf{x}] = \mu \\
\mathrm{cov}[\mathbf{x}] = \mathbf{\Lambda^{-1}}
$$

This is the very form of $p(x)$. Hence the marginal distribution $p(x)$ is
$$
p(\mathbf{x}) = \mathcal{N}(\mathbf{x|}\mu, \mathbf{\Lambda^{-1}})
$$

#### (b)

For the conditional distribution of a multivariate Gaussian, we can utilize the following expressions:
$$
\begin{align*}
\mu_{y|x} &= \mu_y + \Sigma_{yx}\Sigma_{xx}^{-1}(\mathbf{x}-\mu_x) \\
&= \mathbf{A}\mu + \mathbf{b} + \mathbf{A\Lambda^{-1}\Lambda} (\mathbf{x}-\mu) \\
&= \mathbf{Ax} + \mathbf{b}
\end{align*}
$$

$$
\begin{align*}
\Sigma_{y|x} &= \Sigma_{yy} - \Sigma_{yx} \Sigma_{xx}^{-1} \Sigma_{xy} \\
&= \mathbf{L^{-1}+A\Lambda^{-1}A^\mathrm{T}} - \mathbf{A\Lambda^{-1}\Lambda}\mathbf{\Lambda^{-1}A^\mathrm{T}} \\
&= \mathbf{L^{-1}}
\end{align*}
$$

Hence, the conditional distribution $p(\mathbf{y|x})$ is
$$
p(\mathbf{y|x})=\mathcal{N}(\mathbf{y|Ax+b, L^{-1}})
$$

## Question 3

#### maximizes the log likelihood

We have
$$
\frac{\partial}{\partial \mathbf{A}} \mathrm{ln}|\mathbf{A}| = (\mathbf{A^{-1}})^\mathrm{T} \\
\frac{\partial \mathrm{tr}(A\Sigma^{-1})}{\partial \Sigma} = -\Sigma^{-1}A\Sigma^{-1}
$$

$$
\mathbf{z}^\mathrm{T}\Sigma^{-1}\mathbf{z} = \mathrm{tr}(\mathbf{z}^\mathrm{T}\Sigma^{-1}\mathbf{z}) = \mathrm{tr}(\Sigma^{-1}\mathbf{z}\mathbf{z}^\mathrm{T})
$$

$$
\frac{\partial \mathrm{tr}(\Sigma^{-1}\mathbf{z}\mathbf{z}^\mathrm{T})}{\partial \Sigma} = -\Sigma^{-1}\mathbf{z}\mathbf{z}^\mathrm{T}\Sigma^{-1}
$$

Then 

$$
\begin{align*}
\frac{\partial\ln(\mathbf{X}|\mu, \Sigma)}{\partial \Sigma} 
&= -\frac{N}{2} \Sigma^{-T} + \frac{1}{2} \sum^N_{n=1} \Sigma^{-1}(\mathbf{x}_n-\mu)(\mathbf{x}_n-\mu)^T \Sigma^{-1} \\
&= -\frac{N}{2} \Sigma^{-1} + \frac{1}{2} \sum^N_{n=1} \Sigma^{-1}(\mathbf{x}_n-\mu)(\mathbf{x}_n-\mu)^T \Sigma^{-1} \\
&= 0
\end{align*}
$$

It is solved that
$$
\Sigma_{ML} = \frac{1}{N} \sum^N_{n=1}(\mathbf{x}_n-\mu)(\mathbf{x}_n-\mu)^T
$$

#### Symmetric

The transpose of $\Sigma_{ML}$ is:
$$
\Sigma_{ML}^T = \frac{1}{N} \sum^N_{n=1}(\mathbf{x}_n-\mu)^T(\mathbf{x}_n-\mu)
$$
Because $(\mathbf{x}_n-\mu)^T(\mathbf{x}_n-\mu)$â€‹ is scalar, the transpose is itself. Thus we have
$$
\Sigma_{ML} = \Sigma_{ML}^T
$$

#### Positive definition

 If the sample covariance is nonsingular, then it is invertible, which implies it is positive definite.



## Question 4 (a)

$$
\begin{align*}
(\sigma^2_{ML})^{(N)} &= \frac{1}{N}\sum^N_{n=1}(x_n-\mu)^2 \\
&= \frac{1}{N}(x_N-\mu)^2 + \frac{1}{N}\sum^{N-1}_{n=1}(x_n-\mu)^2 \\
&= \frac{1}{N}(x_N-\mu)^2 + \frac{N-1}{N} (\sigma^2_{ML})^{(N-1)}\\
&= (\sigma^2_{ML})^{(N-1)} + \frac{1}{N}\Big((x_N-\mu)^2 - (\sigma^2_{ML})^{(N-1)}\Big)
\end{align*}
$$

$$
\theta^{(N)}=\theta^{(N-1)}-\alpha_{N-1}\frac{\part}{\part{\theta^{(N-1)}}}[-\mathrm{ln}p(x_N|\theta^{(N-1)})]
$$

$$
\begin{align*}
(\sigma^2_{ML})^{(N)} 
&= (\sigma^2_{ML})^{(N - 1)} - \alpha_{N-1} \frac{\partial}{\partial (\sigma^2_{ML})^{(N - 1)}}\left[ -\mathrm{ln}p(x_N|(\sigma^2_{ML})^{(N - 1)}) \right] \\
&= (\sigma^2_{ML})^{(N - 1)} - \alpha_{N-1} \frac{\partial}{\partial (\sigma^2_{ML})^{(N - 1)}}\left[ \frac{1}{2}\ln(2\pi) + \frac{1}{2}\ln(\sigma^2_{ML})^{(N - 1)} + \frac{(x_N - \mu)^2}{2(\sigma^2_{ML})^{(N - 1)}} \right] \\
&= (\sigma^2_{ML})^{(N - 1)} - \alpha_{N-1} \left[ \frac{1}{2(\sigma^2_{ML})^{(N - 1)}} - \frac{(x_N - \mu)^2}{2(\sigma^4_{ML})^{(N - 1)}} \right] \\
&= (\sigma^2_{ML})^{(N - 1)} + \frac{\alpha_{N-1}}{2(\sigma^4_{ML})^{(N - 1)}} \left[ (x_N-\mu)^2 - (\sigma^2_{ML})^{(N-1)} \right]
\end{align*}
$$

Hence, take
$$
\alpha_N=\frac{2(\sigma^{4}_{ML})^{(N)}}{N+1}
$$
to match
$$
(\sigma^2_{ML})^{(N-1)} + \frac{1}{N}\Big((x_N-\mu)^2 - (\sigma^2_{ML})^{(N-1)}\Big)
$$


## Question 4 (b)

$$
\begin{align}
\Sigma^{(N)}_{\mathrm{ML}}&=\frac{1}{N}\sum^N_{n=1}(\mathbf{x}_n-\mu_{\mathrm{ML}})(\mathbf{x}_n-\mu_{\mathrm{ML}})^\mathrm{T}
\\
&=\Sigma^{(N-1)}_{ML}+\frac{1}{N}((\mathbf{x}_N-\mu_{\mathrm{ML}})(\mathbf{x}_N-\mu_{\mathrm{ML}})^\mathrm{T}-\Sigma^{(N-1)}_{ML})
\end{align}
$$

$$
\theta^{(N)}=\theta^{(N-1)}-\alpha_{N-1}\frac{\part}{\part{\theta^{(N-1)}}}[-\mathrm{ln}p(x_N|\theta^{(N-1)})]
$$

$$
\begin{align}
\Sigma^{(N)}_{\mathrm{ML}}&= \Sigma^{(N-1)}_{\mathrm{ML}}-\alpha_{N-1}\frac{\part}{\part{\Sigma^{(N-1)}_{\mathrm{ML}}}}[-\mathrm{ln}p(\mathbf{x}_N|\Sigma^{(N-1)}_{\mathrm{ML}})]
\\&=\Sigma^{(N-1)}_{\mathrm{ML}}-\alpha_{N-1}\frac{\part}{\part{\Sigma^{(N-1)}_{\mathrm{ML}}}}[\frac{ND}{2}\mathrm{ln}(2\pi)+\frac{N}{2}\mathrm{ln}|\Sigma^{(N-1)}_{\mathrm{ML}}|+\frac{1}{2}(\mathbf{x}_N-\mu_{\mathrm{ML}})^\mathrm{T}(\Sigma^{(N-1)}_{\mathrm{ML}})^{-1}(\mathbf{x}_N-\mu_{\mathrm{ML}})]
\\&=\Sigma^{(N-1)}_{\mathrm{ML}}-\alpha_{N-1}[\frac{N}{2}((\Sigma^{(N-1)}_{\mathrm{ML}})^{-1})^\mathrm{T}-\frac{1}{2}(\Sigma^{(N-1)}_{\mathrm{ML}})^{-1}(\mathbf{x}_N-\mu_{\mathrm{ML}})(\mathbf{x}_N-\mu_{\mathrm{ML}})^\mathrm{T}(\Sigma^{(N-1)}_{\mathrm{ML}})^{-1}]
\\&=\Sigma^{(N-1)}_{\mathrm{ML}}-\alpha_{N-1}[\frac{N}{2}((\Sigma^{(N-1)}_{\mathrm{ML}})^{-1})-\frac{1}{2}(\Sigma^{(N-1)}_{\mathrm{ML}})^{-1}(\mathbf{x}_N-\mu_{\mathrm{ML}})(\mathbf{x}_N-\mu_{\mathrm{ML}})^\mathrm{T}(\Sigma^{(N-1)}_{\mathrm{ML}})^{-1}]
\\&=\Sigma^{(N-1)}_{\mathrm{ML}}+\alpha_{N-1}\frac{N}{2}(\Sigma^{(N-1)}_{\mathrm{ML}})^{-1}[\frac{1}{N}((\mathbf{x}_N-\mu_{\mathrm{ML}})(\mathbf{x}_N-\mu_{\mathrm{ML}})^\mathrm{T}-\Sigma^{(N-1)}_{ML})](\Sigma^{(N-1)}_{\mathrm{ML}})^{-1}
\end{align}
$$

Hence, take
$$
\alpha_N=\frac{2\Sigma^{2(N)}_{ML}}{N+1}
$$
to match.



## Question 5

Assume
$$
p(\mu|\mathbf{X})=N(\mu|\mu_N,\Sigma_N)
$$
By Bayesian Inference, 
$$
p(\mu|\mathbf{X}) \propto p(\mathbf{X}|\mu) p(\mu)
$$

$$
-\frac{1}{2}(\mu-\mu_N)^T \Sigma^{-1}_N (\mu-\mu_N) =
\\
\sum^N_{n=1} -\frac{1}{2} (x_n - \mu)^T\Sigma^{-1}(x_n -\mu) - \frac{1}{2}(\mu-\mu_0)^T\Sigma_0^{-1}(\mu - \mu_0)
$$

Then
$$
\begin{align}
\Sigma_N&=N\Sigma^{-1}+\Sigma_0^{-1}
\\\mu_N&=\Sigma_N(\Sigma^{-1}\sum_{n=1}^N\mathbf{x_n}+\Sigma_0^{-1}\mu_0)=(N\Sigma^{-1}+\Sigma_0^{-1})(\Sigma^{-1}\sum_{n=1}^N\mathbf{x_n}+\Sigma_0^{-1}\mu_0)
\end{align}
$$
